fstar/MLS.TreeDEM.KeyPackageRef.fst
@@ -3,12 +3,13 @@ module MLS.TreeDEM.KeyPackageRef
 open Comparse
 open MLS.NetworkTypes
 open MLS.TreeSync.NetworkTypes
+open MLS.TreeKEM.NetworkTypes
 open MLS.TreeDEM.NetworkTypes
 open MLS.Crypto
 open MLS.Result
 
-val compute_key_package_ref: #bytes:Type0 -> {|crypto_bytes bytes|} -> key_package_nt bytes -> result (key_package_ref_nt bytes)
+val compute_key_package_ref: #bytes:Type0 -> {|crypto_bytes bytes|} -> key_package_nt bytes tkt -> result (key_package_ref_nt bytes)
 let compute_key_package_ref #bytes #cb kp =
-  let kp_bytes: bytes = serialize (key_package_nt bytes) kp in
+  let kp_bytes: bytes = serialize (key_package_nt bytes tkt) kp in
   res <-- make_keypackage_ref kp_bytes;
   return (res <: mls_bytes bytes)
