fstar/MLS.TreeSync.Hash.fst
@@ -11,31 +11,31 @@ open MLS.Result
 
 #set-options "--fuel 1 --ifuel 1 --z3rlimit 50"
 
-noeq type leaf_node_tree_hash_input_nt (bytes:Type0) {|bytes_like bytes|} = {
+noeq type leaf_node_tree_hash_input_nt (bytes:Type0) {|bytes_like bytes|} (tkt:treekem_types bytes) = {
   leaf_index: nat_lbytes 4;
-  [@@@ with_parser #bytes (ps_option ps_leaf_node_nt)]
-  leaf_node: option (leaf_node_nt bytes);
+  [@@@ with_parser #bytes (ps_option (ps_leaf_node_nt tkt))]
+  leaf_node: option (leaf_node_nt bytes tkt);
 }
 
 %splice [ps_leaf_node_tree_hash_input_nt] (gen_parser (`leaf_node_tree_hash_input_nt))
 
-noeq type parent_node_tree_hash_input_nt (bytes:Type0) {|bytes_like bytes|} = {
-  [@@@ with_parser #bytes (ps_option ps_parent_node_nt)]
-  parent_node: option (parent_node_nt bytes);
+noeq type parent_node_tree_hash_input_nt (bytes:Type0) {|bytes_like bytes|} (tkt:treekem_types bytes) = {
+  [@@@ with_parser #bytes (ps_option (ps_parent_node_nt tkt))]
+  parent_node: option (parent_node_nt bytes tkt);
   left_hash: mls_bytes bytes;
   right_hash: mls_bytes bytes;
 }
 
 %splice [ps_parent_node_tree_hash_input_nt] (gen_parser (`parent_node_tree_hash_input_nt))
 
-noeq type tree_hash_input_nt (bytes:Type0) {|bytes_like bytes|} =
-  | LeafTreeHashInput: [@@@ with_tag (NT_leaf ())] leaf_node: leaf_node_tree_hash_input_nt bytes -> tree_hash_input_nt bytes
-  | ParentTreeHashInput: [@@@ with_tag (NT_parent ())] parent_node: parent_node_tree_hash_input_nt bytes -> tree_hash_input_nt bytes
+noeq type tree_hash_input_nt (bytes:Type0) {|bytes_like bytes|} (tkt:treekem_types bytes) =
+  | LeafTreeHashInput: [@@@ with_tag (NT_leaf ())] leaf_node: leaf_node_tree_hash_input_nt bytes tkt -> tree_hash_input_nt bytes tkt
+  | ParentTreeHashInput: [@@@ with_tag (NT_parent ())] parent_node: parent_node_tree_hash_input_nt bytes tkt -> tree_hash_input_nt bytes tkt
 
 %splice [ps_tree_hash_input_nt] (gen_parser (`tree_hash_input_nt))
 
-instance parseable_serializeable_tree_hash_input (bytes:Type0) {|bytes_like bytes|}: parseable_serializeable bytes (tree_hash_input_nt bytes) =
-  mk_parseable_serializeable ps_tree_hash_input_nt
+instance parseable_serializeable_tree_hash_input (bytes:Type0) {|bytes_like bytes|} (tkt:treekem_types bytes): parseable_serializeable bytes (tree_hash_input_nt bytes tkt) =
+  mk_parseable_serializeable (ps_tree_hash_input_nt tkt)
 
 val tree_hash: #bytes:Type0 -> {|crypto_bytes bytes|} -> #l:nat -> #i:tree_index l -> treesync bytes l i -> result (lbytes bytes (hash_length #bytes))
 let rec tree_hash #bytes #cb #l #i t =
@@ -51,7 +51,7 @@ let rec tree_hash #bytes #cb #l #i t =
     if not (i < pow2 32) then
       internal_failure "tree_hash: leaf_index too big"
     else
-      hash_hash (serialize (tree_hash_input_nt bytes) (LeafTreeHashInput ({
+      hash_hash (serialize (tree_hash_input_nt bytes MLS.TreeKEM.NetworkTypes.tkt) (LeafTreeHashInput ({
         leaf_index = i;
         leaf_node = leaf_node;
       })))
@@ -65,7 +65,7 @@ let rec tree_hash #bytes #cb #l #i t =
     );
     left_hash <-- tree_hash left;
     right_hash <-- tree_hash right;
-    hash_hash (serialize (tree_hash_input_nt bytes) (ParentTreeHashInput ({
+    hash_hash (serialize (tree_hash_input_nt bytes MLS.TreeKEM.NetworkTypes.tkt) (ParentTreeHashInput ({
       parent_node = parent_node;
       left_hash = left_hash;
       right_hash = right_hash;
