fstar/MLS.TreeSync.IntegrityCheck.fst
@@ -56,8 +56,8 @@ let check_signature #bytes #cb lp group_id =
     let tbs = ({
       data = leaf_node.data;
       group_id = (match leaf_node.data.source with | LNS_commit () | LNS_update () -> group_id | _ -> ());
-    } <: leaf_node_tbs_nt bytes) in
-    let leaf_package_bytes: bytes = serialize (leaf_node_tbs_nt bytes) tbs in
+    } <: leaf_node_tbs_nt bytes MLS.TreeKEM.NetworkTypes.tkt) in
+    let leaf_package_bytes: bytes = serialize (leaf_node_tbs_nt bytes _) tbs in
     signature_ok <-- verify_with_label lp.credential.signature_key (string_to_bytes #bytes "LeafNodeTBS") leaf_package_bytes lp.signature;
     if signature_ok then
       return None
